Update HPKE to fit new spec

code/hpke/Hacl.HPKE.Curve51_CP32_SHA512.fst
@@ -4,15 +4,16 @@ open Hacl.Meta.HPKE
 
 module IDH = Hacl.Impl.Generic.DH
 module IHK = Hacl.Impl.Generic.HKDF
+module IHash = Hacl.Impl.Generic.Hash
 module IAEAD = Hacl.Impl.Instantiate.AEAD
 
 friend Hacl.Meta.HPKE
 
-let setupBaseI = hpke_setupBaseI_higher #cs IHK.hkdf_expand512 IHK.hkdf_extract512 IDH.secret_to_public_c51 IDH.scalarmult_c51
+let setupBaseI = hpke_setupBaseI_higher #cs IHK.hkdf_expand512 IHK.hkdf_extract512 IHash.hash_512 IDH.secret_to_public_c51 IDH.scalarmult_c51
 
-let setupBaseR = hpke_setupBaseR_higher #cs IHK.hkdf_expand512 IHK.hkdf_extract512 IDH.scalarmult_c51 IDH.secret_to_public_c51
+let setupBaseR = hpke_setupBaseR_higher #cs IHK.hkdf_expand512 IHK.hkdf_extract512 IHash.hash_512 IDH.scalarmult_c51 IDH.secret_to_public_c51
 
-let encryptBase = hpke_encryptBase_higher #cs IDH.scalarmult_c51 IDH.secret_to_public_c51
+let sealBase = hpke_sealBase_higher #cs IDH.scalarmult_c51 IDH.secret_to_public_c51
   setupBaseI IAEAD.aead_encrypt_cp32
 
-let decryptBase = hpke_decryptBase_higher #cs IDH.scalarmult_c51 setupBaseR IAEAD.aead_decrypt_cp32
+let openBase = hpke_openBase_higher #cs IDH.scalarmult_c51 setupBaseR IAEAD.aead_decrypt_cp32
